Semantic/Fsub/Eval/BasicProps.lean
@@ -238,6 +238,7 @@ theorem frame_shift_zero (pos : Nat) : frame_shift pos 0 = id := by
   funext n; simp [frame_shift]
 
 theorem step_frame
+  (hwf : Exp.WfIn e1 s1)
   (hr : Step s1 e1 (s1 ++ extra) e2) :
   Step
     (s1 ++ s2)
@@ -246,7 +247,11 @@ theorem step_frame
     (e2.rename_levels (frame_shift s1.len s2.len)) := by
   generalize heq : s1 ++ extra = s_out at hr
   induction hr generalizing s2
-  case st_ctx ih => sorry
+  case st_ctx ih =>
+    obtain ⟨hwf1, hwf2⟩ := Exp.letin_wf_inv hwf
+    subst heq
+    simp [Exp.rename_levels]
+    sorry
   case st_apply => sorry
   case st_tapply => sorry
   case st_rename => sorry
